translator/monadic/ml_monad_translatorLib.sig
@@ -5,8 +5,6 @@ sig
     type monadic_translation_parameters = ml_monadStoreLib.monadic_translation_parameters
     type store_translation_result = ml_monadStoreLib.store_translation_result
 
-    val mem_derive_case_of : hol_type -> thm
-
     (* Functions to initialize the translation *)
     val start_static_init_fixed_store_translation :
 	(string * thm * thm * thm) list ->
@@ -21,7 +19,7 @@ sig
 	string -> hol_type -> thm -> (thm * thm) list -> string list ->
         monadic_translation_parameters * (thm * thm) list
 
-    (* Other functions to initialize the translation - shouldn't be used by the user *)
+    (* Other functions to initialize the translation - the above ones should be preferred *)
     val init_translation :
         monadic_translation_parameters -> thm option -> thm -> string list -> unit
     val add_raise_handle_functions : (thm * thm) list -> thm -> (thm * thm) list
